proofs/common/zmap.v
@@ -1,0 +1,98 @@
+(** This files extends the implementation of finite over [positive] to finite
+maps whose keys range over Coq's data type of binary naturals [Z]. *)
+From stdpp Require Import mapset.
+From stdpp Require Export prelude fin_maps.
+From stdpp Require Import options.
+Require Import pmap countable.
+Local Open Scope Z_scope.
+
+Record Zmap (A : Type) : Type :=
+  ZMap { Zmap_0 : option A; Zmap_pos : Pmap A; Zmap_neg : Pmap A }.
+Add Printing Constructor Zmap.
+Global Arguments Zmap_0 {_} _ : assert.
+Global Arguments Zmap_pos {_} _ : assert.
+Global Arguments Zmap_neg {_} _ : assert.
+Global Arguments ZMap {_} _ _ _ : assert.
+
+Global Instance Zmap_eq_dec `{EqDecision A} : EqDecision (Zmap A).
+Proof.
+ refine (λ t1 t2,
+  match t1, t2 with
+  | ZMap x t1 t1', ZMap y t2 t2' =>
+     cast_if_and3 (decide (x = y)) (decide (t1 = t2)) (decide (t1' = t2'))
+  end); abstract congruence.
+Defined.
+Global Instance Zmap_empty {A} : Empty (Zmap A) := ZMap None ∅ ∅.
+Global Instance Zmap_lookup {A} : Lookup Z A (Zmap A) := λ i t,
+  match i with
+  | Z0 => Zmap_0 t | Zpos p => Zmap_pos t !! p | Zneg p => Zmap_neg t !! p
+  end.
+Global Instance Zmap_partial_alter {A} : PartialAlter Z A (Zmap A) := λ f i t,
+  match i, t with
+  | Z0, ZMap o t t' => ZMap (f o) t t'
+  | Z.pos p, ZMap o t t' => ZMap o (partial_alter f p t) t'
+  | Z.neg p, ZMap o t t' => ZMap o t (partial_alter f p t')
+  end.
+Global Instance Zmap_fmap: FMap Zmap := λ A B f t,
+  match t with ZMap o t t' => ZMap (f <$> o) (f <$> t) (f <$> t') end.
+Global Instance Zmap_omap: OMap Zmap := λ A B f t,
+  match t with ZMap o t t' => ZMap (o ≫= f) (omap f t) (omap f t') end.
+Global Instance Zmap_merge: Merge Zmap := λ A B C f t1 t2,
+  match t1, t2 with
+  | ZMap o1 t1 t1', ZMap o2 t2 t2' =>
+     ZMap (diag_None f o1 o2) (merge f t1 t2) (merge f t1' t2')
+  end.
+Global Instance Zmap_fold {A} : MapFold Z A (Zmap A) := λ B f d t,
+  match t with
+  | ZMap mx t t' => map_fold (f ∘ Z.pos) (map_fold (f ∘ Z.neg)
+     match mx with Some x => f 0 x d | None => d end t') t
+  end.
+
+Global Instance Zmap_map: FinMap Z Zmap.
+Proof.
+  split.
+  - intros ? [??] [??] H. f_equal.
+    + apply (H 0).
+    + apply map_eq. intros i. apply (H (Z.pos i)).
+    + apply map_eq. intros i. apply (H (Z.neg i)).
+  - by intros ? [].
+  - intros ? f [] [|?|?]; simpl; [done| |]; apply lookup_partial_alter.
+  - intros ? f [] [|?|?] [|?|?]; simpl; intuition congruence ||
+      intros; apply lookup_partial_alter_ne; congruence.
+  - intros ??? [??] []; simpl; [done| |]; apply lookup_fmap.
+  - intros ?? f [??] [|?|?]; simpl; [done| |]; apply (lookup_omap f).
+  - intros ??? f [??] [??] [|?|?]; simpl; [done| |]; apply (lookup_merge f).
+  - done.
+  - intros A P Hemp Hins [mx t t'].
+    induction t as [|i x t ? Hfold IH] using map_fold_fmap_ind.
+    { induction t' as [|i x t' ? Hfold IH] using map_fold_fmap_ind.
+      { destruct mx as [x|]; [|done].
+        replace (ZMap (Some x) ∅ ∅) with (<[0:=x]> ∅ : Zmap _) by done.
+        by apply Hins. }
+      apply (Hins (Z.neg i) x (ZMap mx ∅ t')); [done| |done].
+      intros A' B f g b. apply Hfold. }
+    apply (Hins (Z.pos i) x (ZMap mx t t')); [done| |done].
+    intros A' B f g b. apply Hfold.
+Qed.
+
+(** * Finite sets *)
+(** We construct sets of [Z]s satisfying extensional equality. *)
+Notation Zset := (mapset Zmap).
+Global Instance Zmap_dom {A} : Dom (Zmap A) Zset := mapset_dom.
+Global Instance: FinMapDom Z Zmap Zset := mapset_dom_spec.
+
+(*NOTE: NOT in stdpp for some reason*)
+
+Local Definition zmap_to_tup {A} (z: zmap.Zmap A) : option A * pmap.Pmap A * pmap.Pmap A :=
+  (Zmap_0 z, Zmap_pos z, Zmap_neg z).
+Local Definition zmap_of_tup {A} (x: option A * pmap.Pmap A * pmap.Pmap A) : Zmap A :=
+  ZMap (fst (fst x)) (snd (fst x)) (snd x).
+
+Local Lemma zmap_to_tup_inj: forall {A} (x: Zmap A), zmap_of_tup (zmap_to_tup x) = x.
+Proof.
+  intros A [x1 x2 x3]; simpl. reflexivity.
+Qed.
+
+Global Instance zmap_countable {A} `{countable.Countable A} : countable.Countable (zmap.Zmap A) :=
+  inj_countable' zmap_to_tup zmap_of_tup zmap_to_tup_inj.
+
